VCVio.lean
@@ -209,6 +209,7 @@ import VCVio.ProgramLogic.Tactics.Unary
 import VCVio.ProgramLogic.Tactics.Unary.Internals
 import VCVio.ProgramLogic.Unary.Examples
 import VCVio.ProgramLogic.Unary.HandlerSpecs
+import VCVio.ProgramLogic.Unary.HoarePropTriple
 import VCVio.ProgramLogic.Unary.HoareTriple
 import VCVio.ProgramLogic.Unary.SimulateQ
 import VCVio.ProgramLogic.Unary.StdDoBridge
